theory/JITPer_mul_rdx.thy
@@ -74,7 +74,7 @@ lemma mulq_one_step_match_stack2:
   done
 
 lemma encode_aux:"((x64_encode (Pmovq_rr REG_SCRATCH (bpf_to_x64_reg src)) @ x64_encode (Ppushl_r RAX) @ 
-      x64_encode (Pmovq_rr RAX RDX) @ x64_encode (Pmulq_r REG_SCRATCH) @ x64_encode (Pmovq_rr RDX RAX) @ x64_encode (Ppopl RAX)))!0 \<notin> {0xc3, 0xe8}"
+      x64_encode (Pmovq_rr RAX RDX) @ x64_encode (Pimulq_r REG_SCRATCH) @ x64_encode (Pmovq_rr RDX RAX) @ x64_encode (Ppopl RAX)))!0 \<notin> {0xc3, 0xe8}"
  subgoal apply(unfold per_jit_mul_reg64_def x64_encode_def)
    apply(unfold construct_rex_to_u8_def bitfield_insert_u8_def Let_def u8_of_bool_def,simp_all)
    apply(cases "and (u8_of_ireg (bpf_to_x64_reg src)) (8::8 word)",simp_all)
@@ -110,14 +110,14 @@ shows "\<exists> xst'. x64_sem1 1 x64_prog (pc,xst) = (pc',xst') \<and>
       using a5 a6 a8 aux5 per_jit_ins_def by fastforce
     subgoal
       apply (subgoal_tac "the (per_jit_mul_reg64 dst src) = (6, 0, x64_encode (Pmovq_rr R11 (bpf_to_x64_reg src))@(x64_encode (Ppushl_r RAX)) @
-           (x64_encode (Pmovq_rr RAX RDX)) @ (x64_encode (Pmulq_r R11))@ (x64_encode (Pmovq_rr RDX RAX))@ (x64_encode (Ppopl RAX)))")
+           (x64_encode (Pmovq_rr RAX RDX)) @ (x64_encode (Pimulq_r R11))@ (x64_encode (Pmovq_rr RDX RAX))@ (x64_encode (Ppopl RAX)))")
        prefer 2
       subgoal using per_jit_mul_reg64_def a9 by simp
       apply(subgoal_tac "((x64_encode (Pmovq_rr REG_SCRATCH (bpf_to_x64_reg src)) @ x64_encode (Ppushl_r RAX) @ 
-          x64_encode (Pmovq_rr RAX RDX) @ x64_encode (Pmulq_r REG_SCRATCH) @ x64_encode (Pmovq_rr RDX RAX) @ x64_encode (Ppopl RAX)))!1 \<noteq> 0x39")
+          x64_encode (Pmovq_rr RAX RDX) @ x64_encode (Pimulq_r REG_SCRATCH) @ x64_encode (Pmovq_rr RDX RAX) @ x64_encode (Ppopl RAX)))!1 \<noteq> 0x39")
        prefer 2 subgoal apply(unfold per_jit_mul_reg64_def x64_encode_def) by simp
       apply(subgoal_tac "((x64_encode (Pmovq_rr REG_SCRATCH (bpf_to_x64_reg src)) @ x64_encode (Ppushl_r RAX) @ 
-      x64_encode (Pmovq_rr RAX RDX) @ x64_encode (Pmulq_r REG_SCRATCH) @ x64_encode (Pmovq_rr RDX RAX) @ x64_encode (Ppopl RAX)))!0 \<notin> {0xc3, 0xe8}")
+      x64_encode (Pmovq_rr RAX RDX) @ x64_encode (Pimulq_r REG_SCRATCH) @ x64_encode (Pmovq_rr RDX RAX) @ x64_encode (Ppopl RAX)))!0 \<notin> {0xc3, 0xe8}")
       prefer 2 using encode_aux apply simp
       subgoal
         unfolding a3
@@ -132,7 +132,7 @@ shows "\<exists> xst'. x64_sem1 1 x64_prog (pc,xst) = (pc',xst') \<and>
 (* 3.1.1 using consistency to get x64 assembly *)
         apply (subgoal_tac "x64_decode (0::nat)
             (x64_encode (Pmovq_rr REG_SCRATCH (bpf_to_x64_reg src)) @
-             x64_encode (Ppushl_r RAX) @ x64_encode (Pmovq_rr RAX RDX) @ x64_encode (Pmulq_r REG_SCRATCH) @ x64_encode (Pmovq_rr RDX RAX) @ x64_encode (Ppopl RAX))
+             x64_encode (Ppushl_r RAX) @ x64_encode (Pmovq_rr RAX RDX) @ x64_encode (Pimulq_r REG_SCRATCH) @ x64_encode (Pmovq_rr RDX RAX) @ x64_encode (Ppopl RAX))
             = Some (3, Pmovq_rr REG_SCRATCH (bpf_to_x64_reg src))")
          prefer 2
         subgoal
@@ -152,7 +152,7 @@ shows "\<exists> xst'. x64_sem1 1 x64_prog (pc,xst) = (pc',xst') \<and>
         apply (simp only: x64_sem.simps)
         apply (subgoal_tac "x64_decode (3::nat)
             (x64_encode (Pmovq_rr REG_SCRATCH (bpf_to_x64_reg src)) @
-             x64_encode (Ppushl_r RAX) @ x64_encode (Pmovq_rr RAX RDX) @ x64_encode (Pmulq_r REG_SCRATCH) @ x64_encode (Pmovq_rr RDX RAX) @ x64_encode (Ppopl RAX))
+             x64_encode (Ppushl_r RAX) @ x64_encode (Pmovq_rr RAX RDX) @ x64_encode (Pimulq_r REG_SCRATCH) @ x64_encode (Pmovq_rr RDX RAX) @ x64_encode (Ppopl RAX))
             = Some (1, Ppushl_r RAX)")
          prefer 2
 (* this is necessary for later list_in_list_prop_aux2 *)
@@ -182,7 +182,7 @@ shows "\<exists> xst'. x64_sem1 1 x64_prog (pc,xst) = (pc',xst') \<and>
 (* using consistency to get x64 assembly *)
         apply (subgoal_tac "x64_decode (4::nat)
             (x64_encode (Pmovq_rr REG_SCRATCH (bpf_to_x64_reg src)) @
-             x64_encode (Ppushl_r RAX) @ x64_encode (Pmovq_rr RAX RDX) @ x64_encode (Pmulq_r REG_SCRATCH) @ x64_encode (Pmovq_rr RDX RAX) @ x64_encode (Ppopl RAX))
+             x64_encode (Ppushl_r RAX) @ x64_encode (Pmovq_rr RAX RDX) @ x64_encode (Pimulq_r REG_SCRATCH) @ x64_encode (Pmovq_rr RDX RAX) @ x64_encode (Ppopl RAX))
             = Some (3, Pmovq_rr RAX RDX)")
          prefer 2
 (* this is necessary for later list_in_list_prop_aux2 *)
@@ -207,15 +207,15 @@ shows "\<exists> xst'. x64_sem1 1 x64_prog (pc,xst) = (pc',xst') \<and>
 (* using consistency to get x64 assembly *)
         apply (subgoal_tac "x64_decode (7::nat)
             (x64_encode (Pmovq_rr REG_SCRATCH (bpf_to_x64_reg src)) @
-             x64_encode (Ppushl_r RAX) @ x64_encode (Pmovq_rr RAX RDX) @ x64_encode (Pmulq_r REG_SCRATCH) @ x64_encode (Pmovq_rr RDX RAX) @ x64_encode (Ppopl RAX))
-            = Some (3, Pmulq_r REG_SCRATCH)")
+             x64_encode (Ppushl_r RAX) @ x64_encode (Pmovq_rr RAX RDX) @ x64_encode (Pimulq_r REG_SCRATCH) @ x64_encode (Pmovq_rr RDX RAX) @ x64_encode (Ppopl RAX))
+            = Some (3, Pimulq_r REG_SCRATCH)")
          prefer 2
 (* this is necessary for later list_in_list_prop_aux2 *)
         apply (subgoal_tac "length ((x64_encode (Pmovq_rr REG_SCRATCH (bpf_to_x64_reg src)) @
              x64_encode (Ppushl_r RAX) @ x64_encode (Pmovq_rr RAX RDX))) = 7")
          prefer 2 subgoal using x64_encode_def construct_rex_to_u8_def bitfield_insert_u8_def Let_def by simp
         subgoal
-          apply (rule_tac l_bin = "x64_encode (Pmulq_r REG_SCRATCH)" in x64_encode_decode_consistency)
+          apply (rule_tac l_bin = "x64_encode (Pimulq_r REG_SCRATCH)" in x64_encode_decode_consistency)
           subgoal using list_in_list_prop_aux2
             by (metis append_assoc)
           subgoal by simp
@@ -223,7 +223,7 @@ shows "\<exists> xst'. x64_sem1 1 x64_prog (pc,xst) = (pc',xst') \<and>
             by fastforce
           done
         apply simp
-        apply (erule subst [of _ "Some (3::nat, Pmulq_r REG_SCRATCH)"])
+        apply (erule subst [of _ "Some (3::nat, Pimulq_r REG_SCRATCH)"])
         apply (simp add: exec_instr_def)
 (* 3.5 *)
         apply (subgoal_tac "Suc 1 = (2::nat)") prefer 2 subgoal by simp
@@ -232,12 +232,12 @@ shows "\<exists> xst'. x64_sem1 1 x64_prog (pc,xst) = (pc',xst') \<and>
 (* using consistency to get x64 assembly *)
         apply (subgoal_tac "x64_decode (10::nat)
             (x64_encode (Pmovq_rr REG_SCRATCH (bpf_to_x64_reg src)) @
-             x64_encode (Ppushl_r RAX) @ x64_encode (Pmovq_rr RAX RDX) @ x64_encode (Pmulq_r REG_SCRATCH) @ x64_encode (Pmovq_rr RDX RAX) @ x64_encode (Ppopl RAX))
+             x64_encode (Ppushl_r RAX) @ x64_encode (Pmovq_rr RAX RDX) @ x64_encode (Pimulq_r REG_SCRATCH) @ x64_encode (Pmovq_rr RDX RAX) @ x64_encode (Ppopl RAX))
             = Some (3, Pmovq_rr RDX RAX)")
          prefer 2
 (* this is necessary for later list_in_list_prop_aux2 *)
         apply (subgoal_tac "length ((x64_encode (Pmovq_rr REG_SCRATCH (bpf_to_x64_reg src)) @
-             x64_encode (Ppushl_r RAX) @ x64_encode (Pmovq_rr RAX RDX))@ x64_encode (Pmulq_r REG_SCRATCH)) = 10")
+             x64_encode (Ppushl_r RAX) @ x64_encode (Pmovq_rr RAX RDX))@ x64_encode (Pimulq_r REG_SCRATCH)) = 10")
          prefer 2 subgoal using x64_encode_def construct_rex_to_u8_def bitfield_insert_u8_def Let_def by simp
         subgoal
           apply (rule_tac l_bin = "x64_encode (Pmovq_rr RDX RAX)" in x64_encode_decode_consistency)
@@ -257,12 +257,12 @@ shows "\<exists> xst'. x64_sem1 1 x64_prog (pc,xst) = (pc',xst') \<and>
 (* using consistency to get x64 assembly *)
         apply (subgoal_tac "x64_decode (13::nat)
             (x64_encode (Pmovq_rr REG_SCRATCH (bpf_to_x64_reg src)) @
-             x64_encode (Ppushl_r RAX) @ x64_encode (Pmovq_rr RAX RDX) @ x64_encode (Pmulq_r REG_SCRATCH) @ x64_encode (Pmovq_rr RDX RAX) @ x64_encode (Ppopl RAX))
+             x64_encode (Ppushl_r RAX) @ x64_encode (Pmovq_rr RAX RDX) @ x64_encode (Pimulq_r REG_SCRATCH) @ x64_encode (Pmovq_rr RDX RAX) @ x64_encode (Ppopl RAX))
             = Some (1, Ppopl RAX)")
          prefer 2
 (* this is necessary for later list_in_list_prop_aux2 *)
         apply (subgoal_tac "length ((x64_encode (Pmovq_rr REG_SCRATCH (bpf_to_x64_reg src)) @
-             x64_encode (Ppushl_r RAX) @ x64_encode (Pmovq_rr RAX RDX))@ x64_encode (Pmulq_r REG_SCRATCH) @ x64_encode (Pmovq_rr RDX RAX)) = 13")
+             x64_encode (Ppushl_r RAX) @ x64_encode (Pmovq_rr RAX RDX))@ x64_encode (Pimulq_r REG_SCRATCH) @ x64_encode (Pmovq_rr RDX RAX)) = 13")
          prefer 2 subgoal using x64_encode_def construct_rex_to_u8_def bitfield_insert_u8_def Let_def by simp
         subgoal
           apply (rule_tac l_bin = "x64_encode (Ppopl RAX)" in x64_encode_decode_consistency)
